src/BoundedArithmetic/DoubleBoundedProofs.v
@@ -235,6 +235,24 @@ Global Instance decode_mul_double
   : forall x y, tuple_decoder (muldw x y) <~=~> (decode x * decode y)%Z
   := proj1 decode_mul_double_iff _.
 
+
+Lemma ripple_carry_tuple_SS' {T} f k xss yss carry
+  : @ripple_carry_tuple T f (S (S k)) xss yss carry
+    = let '(xs, x) := xss in
+      let '(ys, y) := yss in
+      let '(carry, zs) := (@ripple_carry_tuple _ f (S k) xs ys carry) in
+      let '(carry, z) := (f x y carry) in
+      (carry, (zs, z)).
+Proof. reflexivity. Qed.
+
+Local Ltac eta_expand :=
+  repeat match goal with
+         | _ => rewrite !unlock_let
+         | [ |- context[let '(x, y) := ?e in _] ]
+           => rewrite (surjective_pairing e)
+         | _ => rewrite <- !surjective_pairing
+         end.
+
 Lemma ripple_carry_tuple_SS {T} f k xss yss carry
   : @ripple_carry_tuple T f (S (S k)) xss yss carry
     = let '(xs, x) := eta xss in
@@ -242,7 +260,11 @@ Lemma ripple_carry_tuple_SS {T} f k xss yss carry
       let '(carry, zs) := eta (@ripple_carry_tuple _ f (S k) xs ys carry) in
       let '(carry, z) := eta (f x y carry) in
       (carry, (zs, z)).
-Proof. reflexivity. Qed.
+Proof.
+  rewrite ripple_carry_tuple_SS'.
+  eta_expand.
+  reflexivity.
+Qed.
 
 Lemma carry_is_good (n z0 z1 k : Z)
   : 0 <= n ->
@@ -414,7 +436,7 @@ Section tuple2.
     Proof.
       assert (0 <= 2 * half_n) by eauto using decode_exponent_nonnegative.
       assert (0 <= half_n) by omega.
-      unfold mul_double.
+      unfold mul_double; eta_expand.
       push_decode; autorewrite with simpl_tuple_decoder; simplify_projections.
       autorewrite with zsimplify Zshift_to_pow push_Zpow.
       rewrite !spread_left_from_shift_half_correct.
